#### Esercizio 1
$\overline A \cdot (A+B)+\overline C+BC=B+\overline C$ 
#### Esercizio 2
$\overline {A+A \overline B+CD}=\overline A (\overline C+ \overline D)$
#### Esercizio 3
$\overline B \cdot \overline C+ AB \overline C=\overline B \cdot \overline C+ A \overline C$
#### Esercizio 4
$\overline A \cdot \overline B \cdot \overline C+ A \cdot \overline B \cdot \overline C+\overline A \cdot B \cdot \overline C+A \cdot B \cdot \overline C=\overline C$
#### Esercizio 5
$\overline{\overline{AB}+C \overline D}=AB \overline C+ABD$
#### Esercizio 6
$A \overline BC+\overline A \ \overline C D+ A \overline C=A \overline B+ A \overline C+\overline CD$
#### Esercizio 7
$BC\overline D+CD+A \overline B C \overline D+ \overline A \overline BC=C$
#### Esercizio 8
$\overline{\overline A + ABC}=A(\overline B + \overline C)$
#### Esercizio 9
$(A+B)(A+\overline B)=A$
#### Esercizio 10
$C+B \cdot \overline{A+B} \cdot \overline{\overline A \cdot \overline C}+B=C+B$
#### Esercizio 11
$\overline{ABC + A} + B=\overline A + B$
#### Esercizio 12
$(A+B+\overline C+D)(A+\overline B+ \overline C+ D)(A+\overline B+ \overline C+ \overline D)=A+\overline C+ D \overline B$
#### Esercizio 13
$\overline{\overline{A+C}+\overline A+ \overline B}+\overline{BC+\overline B \ \overline C+AB+\overline A \ \overline B}=A \overline B+ \overline A B+\overline A C$
